[hott] definition of pointed type and loop spaces

hott/intro.v
@@ -1,7 +1,7 @@
 Inductive paths {A} : A -> A -> Type :=
   idpath : forall x, paths x x.
 
-Notation "x ~> y" := (paths x y) (at level 70).
+Notation "x <~> y" := (paths x y) (at level 70).
 
 Hint Resolve idpath.
 
@@ -9,37 +9,37 @@ Check paths_ind.
 
 Definition ind :
   forall A
-         (D : forall (x y : A), (x ~> y) -> Type),
+         (D : forall (x y : A), (x <~> y) -> Type),
          (forall (a : A), D a a (idpath a)) ->
-         forall (x y : A) (p : (x ~> y)), D x y p.
+         forall (x y : A) (p : (x <~> y)), D x y p.
 Proof.
   intros.
   induction p.
   apply X.
 Defined.
 
-Definition inv: forall {A} {x y : A}, (x ~> y) -> (y ~> x).
+Definition inv: forall {A} {x y : A}, (x <~> y) -> (y <~> x).
 Proof.
   intros.
   induction X.
   apply idpath.
 Defined.
 
-Lemma inv_inv : forall {A} {x y : A} {p : x ~> y}, inv (inv p) ~> p.
+Definition inv_inv : forall {A} {x y : A} {p : x <~> y}, inv (inv p) <~> p.
 Proof.
   intros.
   induction p.
   unfold inv. simpl.
   apply idpath.
-Qed.
+Defined.
 
-Definition concat: forall {A} {x y z : A}, (x ~> y) -> (y ~> z) -> (x ~> z) :=
+Definition concat: forall {A} {x y z : A}, (x <~> y) -> (y <~> z) -> (x <~> z) :=
   fun A x y z xy yz =>
     ind A
-        (fun x y p => forall (z: A), (y ~> z) -> (x ~> z))
+        (fun x y p => forall (z: A), (y <~> z) -> (x <~> z))
         (fun a =>
            ind A
-               (fun x y xy => x ~> y)
+               (fun a b _ => a <~> b)
                (fun w => idpath w)
                a
         )
@@ -50,20 +50,56 @@ Print concat.
 
 Notation "p @ q" := (concat p q) (at level 60).
 
-Lemma concat_idpath : forall A {x: A}, concat (idpath x) (idpath x) = idpath x.
+Lemma concat_idpath : forall A {x: A}, (idpath x) @ (idpath x) = idpath x.
 Proof.
   intros.
   simpl.
   reflexivity.
 Qed.
 
-(* It's very weird that concat defined in Proof mode will be un-expandable. *)
+(* It's very weird that concat defined in Proof mode will be
+   un-expandable.  Proof. ... Qed. marks the definition
+   opaque. Whereas Proof. ... Defined. marks the definition
+   transparent.
+  *)
 
 Notation "! p" := (inv p) (at level 50).
 
-Definition idpath_left_unit : forall A (x y : A) (p : x ~> y), (idpath x @ p) ~> p.
+Definition idpath_left_unit : forall A (x y : A) (p : x <~> y), (idpath x @ p) <~> p.
 Proof.
   intros.
   induction p.
   auto.
 Qed.
+
+Definition idpath_right_unit : forall A (x y : A) (p : x <~> y), (p @ idpath y) <~> p.
+Proof.
+  intros.
+  induction p.
+  auto.
+Qed.
+
+Require Import Coq.Init.Nat.
+
+Inductive pointed A (a : A) : Type :=
+| point_intro : pointed A a.
+
+Hint Resolve point_intro.
+
+Definition loop A (a : A) : Type := (pointed (a <~> a) (idpath a)).
+
+Print loop.
+
+Definition loop_concat A (a : A) (x : loop A a) (y : loop A a) : loop A a.
+Proof. trivial. Qed.
+
+Print loop_concat.
+
+Definition loop2 A (a : A) : Type := loop (loop A a) (point_intro _ _).
+Print loop2.
+
+(*
+loop2 =
+fun (A : Type) (a : A) => loop (loop A a) (point_intro (a <~> a) (idpath a))
+     : forall A : Type, A -> Type
+ *)
